Fixed Lecture_04/.ec. Brainstorming about superduniform.

lecture-files-fixed/Lecture_04/Lecture.ec
@@ -3,11 +3,17 @@ require import AllCore.
 (* import Fun.Bijections. *)
 require FSet.
 (* require ISet. *)
+require Distr.
 
 (* print FSet.Duni.duni . *)
 
 type D.
-(* axiom finD: ISet.Finite.finite ISet.univ<:D>. *)
+clone Distr.MFinite as DD with
+  type t <= D.
+(* Implicitly axiomatized finiteness: *)
+print DD.Support.enum_spec.
+(* If we wanted not to axiomatize it, we would add "proof *" before the . in the clone command *)
+
 op f : D -> D.
 axiom f_bij: bijective f.
 axiom no_fix x: f x <> x.
@@ -17,9 +23,9 @@ module Game = {
     var x : D;
     var x' : D;
     var y : D;
-    x <$ FSet.Duni.duni (ISet.Finite.toFSet ISet.univ<:D>); (* x uniform in D *)
-    y = f (x);  (* x := f x *)
-    x' = y; (* Adv returns x':=y *)
+    x <$ DD.dunifin; (* x uniform in D *)
+    y <- f (x);  (* x := f x *)
+    x' <- y; (* Adv returns x':=y *)
     return x=x';
   }
 }.
@@ -41,9 +47,9 @@ module Game2 = {
     var x : D;
     var x' : D;
     var y : D;
-    x = $ FSet.Duni.duni (ISet.Finite.toFSet ISet.univ<:D>); (* x uniform in D *)
-    y = f x;  (* x := f x *)
-    x' = f y; (* Adv returns x':=f(y) *)
+    x <$ DD.dunifin; (* x uniform in D *)
+    y <- f x;  (* x := f x *)
+    x' <- f y; (* Adv returns x':=f(y) *)
     return x=x';
   }
 }.
@@ -54,4 +60,63 @@ lemma adv_silly2:
     hoare [ Game2.owp : true ==> res<>true ].
 proof.
   proc; auto; smt.
+qed.
+
+import List.
+import Distr.
+print duniform.
+lemma test (x:'a): mu1 (duniform []) x = 0%r.
+    smt.
+qed.
+
+lemma test2 (x:'a) l:
+    (x \in l)%List =>
+    mu1 (duniform l) x > 0%r.
+    smt.
+qed.
+
+type 'a set = 'a -> bool.
+
+op superduniform (s : 'a set) : 'a distr =
+  duniform (choiceb (fun l => s = List.mem l) []).
+
+
+op finite (s: 'a set) : bool =
+  exists l, s = List.mem l.
+
+(* lemma finlist (s:'a set): *)
+(*     finite s => exists l, s = List.mem l. *)
+(*   smt. *)
+(* qed. *)
+
+lemma link (l:'a list):
+    duniform l = superduniform (List.mem l).
+    rewrite /superduniform.
+    pose l0 := choiceb (fun (l0 : 'a list) => mem l = mem l0) [].
+    rewrite -eq_duniformP.
+    have Hl0: mem l = mem l0.
+    smt.
+    rewrite Hl0.
+    trivial.
+qed.
+    
+lemma test3 (x:'a) s:
+    finite s =>
+    s x =>
+    mu1 (superduniform s) x > 0%r.
+    
+    move => Hfin Hmem.
+    have Hex: exists l, s = List.mem l.
+    rewrite /finite in Hfin.
+    apply Hfin.
+    elim Hex.
+
+    move => l Hl.
+    rewrite Hl.
+    rewrite -link.
+
+    apply test2.
+    rewrite -Hl.
+    apply Hmem.
+
 qed.
